low/RinternalsAux.v
@@ -386,6 +386,14 @@ Proof. apply prove_Inhab. repeat constructors. Qed.
 Instance double_Inhab : Inhab double.
 Proof. apply prove_Inhab. repeat constructors. Qed.
 
-Instance RComplex_Inhab : Inhab RComplex.
+Instance Rcomplex_Inhab : Inhab Rcomplex.
 Proof. apply prove_Inhab. repeat constructors. Qed.
 
+(* Warning: this is using the Leibniz equality, not the usual “equality operator” on floats. *)
+Instance double_comparable : Comparable double.
+  prove_comparable_simple_inductive.
+Defined.
+
+Instance Rcomplex_comparable : Comparable Rcomplex.
+  prove_comparable_simple_inductive.
+Defined.
